verified "simplified" nondet

lawyer/examples/nondet/nondet_adequacy.v
@@ -80,4 +80,147 @@ Section NondetAdequacy.
     rewrite START. by iApply closed_pre_helper.
   Qed.
 
+  Definition conf_init_pre (cnt flag: loc) := ([stop_and_read #cnt #flag; incr_loop #cnt #flag], Build_state {[ cnt := #0; flag := #false ]} ∅). 
+
+  Definition δ_init_pre: ProgressState := 
+      {| ps_cps := 30 *: {[+ (π0, d0) +]};
+         ps_sigs := {[ 0 := (tt, false) ]};
+         ps_obls := {[ 0 := {[ 0 ]}; 1 := ∅ ]};
+         ps_eps := {[ (0, π0, d0) ]};
+         ps_phases := {[ 0 := ext_phase π0 0; 1 := ext_phase π0 1 ]};
+         ps_exc_bound := 30 |}. 
+
+  Lemma init_pre_is_init cnt flag:
+    obls_is_init_st (conf_init_pre cnt flag) δ_init_pre.
+  Proof using.
+    rewrite /conf_init_pre /δ_init_pre. 
+    repeat split; simpl. 
+    - red. simpl. set_solver.
+    - simpl in *. repeat rewrite lookup_insert_Some in H0, H1.
+      destruct H0 as [[<- <-] | [? [[<- <-] | [? ?]]]], H1 as [[<- <-] | [? [[<- <-] | [? ?]]]].
+      all: try set_solver.
+      all: by apply obligations_wf.ext_phase_not_le.
+    - simpl in *. repeat rewrite lookup_insert_Some in H0, H1.
+      destruct H0 as [[<- <-] | [? [[<- <-] | [? ?]]]], H1 as [[<- <-] | [? [[<- <-] | [? ?]]]].
+      all: try set_solver.
+      all: by apply obligations_wf.ext_phase_not_le.
+    - red. simpl. intros (?&?&?& IN&IN'&LT).
+      repeat rewrite lookup_insert_Some in IN.
+      apply gmultiset_elem_of_scalar_mul in IN' as (?&IN').
+      apply gmultiset_elem_of_singleton in IN'. subst.
+      simpl in LT.
+      destruct IN as [[<- <-] | [? [[<- <-] | [? ?]]]]; try set_solver.
+      all: apply strict_spec in LT as (_&LT); apply LT; apply phase_lt_fork. 
+    - red. simpl. intros (?&?&?& IN&IN'&LT).
+      repeat rewrite lookup_insert_Some in IN.
+      apply elem_of_singleton in IN'. subst.
+      simpl in LT.
+      destruct IN as [[<- <-] | [? [[<- <-] | [? ?]]]]; try set_solver.
+      all: apply strict_spec in LT as (_&LT); apply LT; apply phase_lt_fork.
+    - red. simpl. set_solver.
+    - red. simpl. intros.
+      destruct τ1 as [|[|]], τ2 as [|[|]]; simpl; try set_solver.
+      + rewrite lookup_insert. repeat (rewrite lookup_insert_ne; [| done]).
+        set_solver. 
+      + do 1 (rewrite lookup_insert_ne; [| done]).
+        rewrite lookup_singleton_ne; [| done].
+        set_solver. 
+      + do 3 (rewrite lookup_insert_ne; [| done]). done.
+  Qed.
+
+  Lemma init_live_tids cnt flag:
+    obls_fairness_preservation.om_live_tids id locale_enabled
+      (conf_init_pre cnt flag) δ_init_pre.
+  Proof using.
+    rewrite /conf_init_pre /δ_init_pre.
+    red. rewrite /has_obls /locale_enabled. simpl.
+    intros ?. destruct ζ as [|[|]].
+    - rewrite lookup_insert. intros _.
+      eexists _. simpl.
+      rewrite from_locale_lookup. simpl. eauto.
+    - rewrite lookup_insert_ne; [| done]. rewrite lookup_insert.
+      set_solver.
+    - repeat (rewrite lookup_insert_ne; [| done]). set_solver. 
+  Qed.
+
+  Theorem nondet_pre_allocated_termination
+    (extr : heap_lang_extrace)    
+    (cnt: loc := Loc 15) (flag: loc := Loc 47) (** arbitrary locations for counter and flag*)
+    (START: trfirst extr = conf_init_pre cnt flag)
+    (VALID: extrace_valid extr):
+    extrace_fairly_terminating extr.
+  Proof.
+    assert (heapGpreS NDΣ EM) as HPreG.
+    { apply subG_heapPreG.
+      apply _. }
+    
+    eapply @obls_terminates_impl_multiple with
+      (δ := δ_init_pre); eauto.
+    1-2: by apply _.
+    { apply unit_WF. }
+    { apply fin_wf. }
+    { simpl. lia. }
+    { apply init_pre_is_init. }
+    { apply init_live_tids. }
+
+    iIntros (?) "[HEAP INIT]". simpl.
+    rewrite big_sepM_insert.
+    2: { rewrite lookup_insert_ne; done. }
+    rewrite big_sepM_singleton.
+    iDestruct "HEAP" as "[CNT FLAG]".
+
+    rewrite /obls_init_resource. iDestruct "INIT" as "(CPS & SIGS & OBS & #EPS & PHS & #EB)".
+    simpl. rewrite /sig_map_repr /obls_map_repr. simpl.
+    rewrite map_fmap_singleton. rewrite !fmap_insert fmap_empty insert_empty.   
+
+    replace #0 with #0%nat by done.
+
+    rewrite insert_union_singleton_l. rewrite -gmap_op_union.
+    2: { apply map_disjoint_dom. set_solver. }
+    rewrite auth_frag_op own_op. iDestruct "OBS" as "[OB0 OB1]".
+    pose proof @alloc_nondet_inv_impl.
+    specialize (H _ _ _ ND_OP_HL _ EM NDΣ (OHE HEAP) () 0 _ 0 cnt flag 0).
+
+    iApply fupd_mask_mono; [apply empty_subseteq| ]. 
+    iMod (H with "[$] [$] [$] [$] []") as "foo".
+    { iApply (exc_lb_le with "[$]"). lia. }
+    iDestruct "foo" as (ND) "(#INV & OB0 & #SGN' & TOK)".
+    iModIntro. rewrite bi.sep_assoc. iSplit; [| done].
+    rewrite big_sepM_insert.
+    2: { rewrite lookup_insert_ne; done. }
+    rewrite big_sepM_singleton. iDestruct "PHS" as "[PH0 PH1]".
+    pose proof (cp_mul_alt π0 d0 30). rewrite -H0. clear H0.
+    replace 30 with (15 + 15) by lia. iDestruct (cp_mul_split with "CPS") as "[CPS0 CPS1]". 
+    iSplitL "OB0 PH0 CPS0 TOK".
+    - pose proof @stop_and_read_spec as SPEC. 
+      specialize SPEC with (OHE := OHE HEAP) (d0 := d0) (d1 := d1) (l__f := ()).
+      iApply (SPEC with "[-]").
+      { apply ith_bn_lt; lia. }
+      { (** for nondet as the closed program, K is irrelevant *)
+        apply le_0_n. }
+      { simpl. iIntros (? _) "X". iApply "X". }
+      { lia. }
+      2: { simpl. iNext. iIntros (?) "(%&% &?&?&?&?)". iFrame. }
+      iFrame "INV PH0 TOK SGN' OB0".      
+      iSplitR. 
+      + iApply (exc_lb_le with "[$]"). lia.
+      + iApply (cp_mul_weaken with "[$]").
+        * apply phase_lt_fork.
+        * lia.
+    - pose proof @incr_loop_spec as SPEC. 
+      specialize SPEC with (OHE := OHE HEAP) (d0 := d0) (l__f := ()).
+      iApply (SPEC with "[-]").
+      4: { by iIntros "!> % ?". }
+      2: lia.
+      2: iFrame "INV PH1 OB1".
+      { lia. }
+      iSplitL. 
+      + iApply (cp_mul_weaken with "[$]").
+        * apply phase_lt_fork.
+        * lia.
+      + rewrite /eps_repr.
+        rewrite /ep. iExists _. iFrame "EPS".
+        iPureIntro. apply phase_lt_fork.
+  Qed.
+
 End NondetAdequacy.
